src/RewriterInterpProofs1.v
@@ -5,7 +5,6 @@ Require Import Coq.Lists.List.
 Require Import Coq.Classes.Morphisms.
 Require Import Coq.MSets.MSetPositive.
 Require Import Coq.FSets.FMapPositive.
-Require Import Coq.Logic.FunctionalExtensionality.
 Require Import Crypto.Language.
 Require Import Crypto.LanguageInversion.
 Require Import Crypto.LanguageWf.
